x86/RawAsmproof.v
@@ -568,6 +568,26 @@ Qed.
       repeat simpl_inject. econstructor; eauto. rewrite Ptrofs.add_zero. auto.
     Qed.
 
+    Lemma goto_ofs_inject:
+      forall j g rs1 rs2 m1 m2
+        (GLOBFUN_INJ: forall b f, Genv.find_funct_ptr ge b = Some f -> j b = Some (b,0))
+        (MINJ: Mem.inject j g m1 m2)
+        (RINJ : forall r : PregEq.t, Val.inject j (rs1 r) (rs2 r))
+        sz ofs rs1' m1',
+        goto_ofs ge sz ofs rs1 m1 = Next rs1' m1' ->
+        exists rs2' m2',
+          goto_ofs ge sz ofs rs2 m2 = Next rs2' m2' /\
+          Mem.inject j g m1' m2' /\
+          forall r, Val.inject j (rs1' r) (rs2' r).
+    Proof.
+      unfold goto_ofs. intros. repeat destr_in H.
+      generalize (RINJ PC); rewrite Heqv. intro A; inv A.
+      erewrite GLOBFUN_INJ in H2; eauto. inv H2. rewrite Heqo.
+      do 2 eexists; split; eauto. split; eauto.
+      repeat simpl_inject. econstructor; eauto. repeat rewrite Ptrofs.add_zero. auto.
+    Qed.
+
+
     Lemma eval_ros_inject:
       forall j rs1 rs2
         (MPG: meminj_preserves_globals' ge j)
@@ -687,7 +707,33 @@ Qed.
     rewrite Heqo.
     eapply goto_label_inject; eauto.
     repeat simpl_inject.
+
+    eapply goto_ofs_inject; eauto.
+
+    erewrite eval_testcond_inject; eauto. simpl.
+    eapply goto_ofs_inject; eauto.
+    erewrite eval_testcond_inject; eauto. simpl.
+    do 2 eexists; split; eauto. split; eauto. repeat simpl_inject.
+
+    erewrite eval_testcond_inject; eauto. simpl.
+    erewrite eval_testcond_inject; eauto. simpl.
+    eapply goto_ofs_inject; eauto.
+
+    erewrite eval_testcond_inject; eauto. simpl.
+    erewrite eval_testcond_inject; eauto. simpl.
+    do 2 eexists; split; eauto. split; eauto. repeat simpl_inject.
+
+    erewrite eval_testcond_inject; eauto. simpl.
+    erewrite eval_testcond_inject; eauto. simpl.
+    do 2 eexists; split; eauto. split; eauto. repeat simpl_inject.
+
+    generalize (RINJ r); rewrite Heqv; intro A; inv A.
+    rewrite Heqo.
+    eapply goto_ofs_inject; eauto.
+    repeat simpl_inject.
+
   Qed.
+
   (* should be proved already somewhere *)
   
   Lemma ZEQ: forall a b,
